\question Prove that $$\sum_{i=0}^{n} i \cdot i! = (n+1)! - 1$$  for 
$n \geq 1$ where $n \in N$.
\begin{solution}[3in]

\textit{Base case}: For $n = 1$, we get 
\[0 \cdot  0! + 1 \cdot 1! = 0 + 1 = 1 = (1 + 1)! - 1 = 2 - 1,\] which is true 
as $1 = 1$.

\textit{Induction Hypothesis}: Assume the following is true for some $k$. 
\[\sum_{i=0}^{k} i \cdot i! = (k+1)! - 1\] 

\textit{Inductive Step}: Let's prove this for  $k + 1$.
\begin{align*}
\sum_{i = 0}^{k + 1} i \cdot  i! &= \sum_{i = 1}^k i \cdot  i! + (k + 1) \cdot (k + 1)! \\
&= (k + 1)! - 1 + (k+1)(k+1)!\\
\intertext{by the inductive hypothesis,}
&= (k + 1)!(1 + k + 1) - 1 \\
&= (k + 1)!(k + 2) - 1 \\
&= (k + 2)! - 1
\end{align*}
Hence, we have proven it for $k+1$, and it is true for all $n$.
\end{solution}

\clearpage
